.

theories/System/Lang.v
@@ -1,4 +1,5 @@
 Require Import PnV.Prelude.Prelude.
+Require Import PnV.Prelude.ConstructiveFacts.
 Require Import PnV.Math.ThN.
 Require Import PnV.System.P.
 
@@ -12,7 +13,7 @@ Variant alphabet : Set :=
 #[local] Notation lang := (ensemble string).
 #[local] Infix " \in " := E.In : type_scope.
 
-#[local]
+#[global]
 Instance alphabet_hasEqDec
   : hasEqDec alphabet.
 Proof.
@@ -148,7 +149,7 @@ Proof with eauto.
     destruct count_L_s_lt_count_R_s as [[? ? ? ? ?] | H_last_R].
     + assert (IH1 : length s' < S (length s)) by now pose proof (@length_app _ s_prefix s'); subst s; lia.
       pose proof (IHs s' IH1 H_cut) as H_s'.
-      assert (IH2: length (L :: s_prefix) < S (length s)) by now simpl; pose proof (@length_app _ s_prefix s'); subst s; lia.
+      assert (IH2 : length (L :: s_prefix) < S (length s)) by now simpl; pose proof (@length_app _ s_prefix s'); subst s; lia.
       assert (CLAIM : count L (L :: s_prefix) = count R (L :: s_prefix)).
       { eapply count_app_cancel_r with (s := L :: s_prefix) (s' := s') (n' := count R s')...
         simpl. rewrite <- H_app. rewrite <- count_app. rewrite <- H_app...
@@ -197,20 +198,11 @@ End LANG1.
 
 Module LANG2.
 
-Variant alphabet : Set :=
-  | L
-  | R.
+Import LANG1.
 
 #[local] Notation string := (list alphabet).
 #[local] Notation lang := (ensemble string).
 #[local] Infix " \in " := E.In : type_scope.
-
-#[local]
-Instance alphabet_hasEqDec
-  : hasEqDec alphabet.
-Proof.
-  red. decide equality.
-Defined.
 
 Inductive L_cfg2 : lang :=
   | cfg2_epsilon
@@ -218,13 +210,252 @@ Inductive L_cfg2 : lang :=
   | cfg2_paren str
     (H_cfg2 : str \in L_cfg2)
     : [L] ++ str ++ [R] \in L_cfg2
-  | cfg2_app str1 str2
+  | cfg2_concat str1 str2
     (H1_cfg2 : str1 \in L_cfg2)
     (H2_cfg2 : str2 \in L_cfg2)
     : str1 ++ str2 \in L_cfg2.
 
+Section THEORY.
+
 #[local] Hint Constructors L_cfg2 : core.
 
 #[local] Notation count a s := (count_occ eq_dec s a).
+
+Lemma count_L_sum_count_R s
+  : count L s + count R s = length s.
+Proof.
+  induction s as [ | [ | ] s IHs]; simpl; lia.
+Qed.
+
+Inductive isPrefixOf (s_prefix : string) : string -> Prop :=
+  | isPrefixOf_intro s_suffix
+    : isPrefixOf s_prefix (s_prefix ++ s_suffix).
+
+#[local] Infix "\prefix" := isPrefixOf (at level 70, no associativity) : type_scope.
+
+#[local] Hint Constructors isPrefixOf : simplication_hints.
+
+#[local] Hint Rewrite length_app length_firstn : simplication_hints.
+
+#[global]
+Instance isPrefixOf_Reflexive
+  : Reflexive isPrefixOf.
+Proof.
+  intros s. rewrite <- app_nil_r with (l := s) at 2. econs.
+Qed.
+
+#[global]
+Instance isPrefixOf_Transitive
+  : Transitive isPrefixOf.
+Proof.
+  intros s1 s2 s3 H12 H23. inv H23. inv H12. rewrite <- app_assoc. econs.
+Qed.
+
+#[global]
+Instance isPrefixOf_Antisymmetric
+  : Antisymmetric string eq isPrefixOf.
+Proof.
+  intros s1 s2 H12 H21.
+  inv H12. rename s_suffix into s2.
+  inv H21. rename s_suffix into s3.
+  pose proof (f_equal (@length alphabet) H) as HH.
+  destruct s2, s3; ss!.
+Qed.
+
+Lemma app_isPrefixOf s s1 s2
+  (PREFIX : s1 \prefix s2)
+  : s ++ s1 \prefix s ++ s2.
+Proof.
+  inv PREFIX. rewrite -> app_assoc. econs.
+Qed.
+
+Lemma firstn_isPrefixOf n s
+  : L.firstn n s \prefix s.
+Proof.
+  rewrite <- firstn_skipn with (n := n) (l := s) at 2. econs.
+Qed.
+
+Lemma isPrefixOf_inv {s : string} {s1 : string} {s2 : string}
+  (H_prefix : s \prefix s1 ++ s2)
+  : {s \prefix s1} + {exists s', s = s1 ++ s' /\ length s' > 0 /\ s' \prefix s2}.
+Proof.
+  destruct (Nat.leb (length s) (length s1)) as [ | ] eqn: H_OBS.
+  - left. rewrite Nat.leb_le in H_OBS. inv H_prefix.
+    pose proof (f_equal (firstn (length s)) H0) as HH.
+    rewrite firstn_app in HH. replace (length s - length s)%nat with 0%nat in HH by lia.
+    rewrite firstn_0 in HH. rewrite app_nil_r in HH. rewrite firstn_all in HH.
+    rewrite firstn_app in HH. replace (length s - length s1)%nat with 0%nat in HH by lia.
+    rewrite firstn_0 in HH. rewrite app_nil_r in HH. rewrite HH. eapply firstn_isPrefixOf.
+  - right. rewrite Nat.leb_nle in H_OBS. inv H_prefix.
+    pose proof (f_equal (firstn (length s)) H0) as HH.
+    rewrite firstn_app in HH. replace (length s - length s)%nat with 0%nat in HH by lia.
+    rewrite firstn_0 in HH. rewrite app_nil_r in HH. rewrite firstn_all in HH.
+    rewrite firstn_app in HH. rewrite firstn_all2 with (l := s1) (n := length s) in HH by lia.
+    exists (L.firstn (length s - length s1)%nat s2). repeat rewrite length_firstn.
+    split; eauto. split.
+    + pose proof (f_equal (@length alphabet) HH) as HH'. s!. lia.
+    + pose proof (COPY := H0). rewrite HH in COPY. rewrite <- app_assoc in COPY.
+      apply L.app_cancel_l with (prefix := s1) in COPY. rewrite <- COPY at 2. econs.
+Qed.
+
+Variant WellParen (s : string) : Prop :=
+  | WellParen_intro
+    (count_L_eq_count_R : count L s = count R s)
+    (PREFIX : forall s_prefix, forall H_prefix : s_prefix \prefix s, count L s_prefix >= count R s_prefix).
+
+Variant WellParen' (s : string) : Prop :=
+  | WellParen'_intro
+    (count_L_eq_count_R : count L s = count R s)
+    (PREFIX : forall prefix, length prefix > 0 -> forall suffix, length suffix > 0 -> [L] ++ s ++ [R] = prefix ++ suffix -> count L prefix > count R prefix).
+
+#[local] Hint Rewrite count_app app_assoc length_app app_nil_r : simplication_hints.
+
+Lemma WellParen_iff_WellParen' s
+  : WellParen s <-> WellParen' s.
+Proof with eauto.
+  split; intros [? ?].
+  - econs... intros ? POS ? POS' H.
+    destruct prefix as [ | [ | ] prefix]; s!; cycle -1.
+    { congruence. }
+    { exfalso; lia. }
+    induction suffix as [ | [ | ] suffix _] using rev_ind; s!.
+    { exfalso. lia. }
+    { enough (R = L) by congruence.
+      assert (H_view : R = last (L :: s ++ [R]) R).
+      { rewrite L.last_cons. rewrite L.last_last... }
+      assert (H_view' : L = last (L :: (prefix ++ suffix) ++ [L]) R).
+      { rewrite L.last_cons. rewrite L.last_last... }
+      congruence.
+    }
+    { apply L.app_cancel_l with (prefix := [L]) in H.
+      apply L.app_cancel_r with (suffix := [R]) in H.
+      exploit (PREFIX prefix); ss!.
+    }
+  - split... intros ? H_prefix; inversion H_prefix.
+    rename s_prefix into s1, s_suffix into s2. subst s.
+    enough (count L ([L] ++ s1) > count R ([L] ++ s1)) by ss!.
+    eapply PREFIX with (prefix := [L] ++ s1) (suffix := s2 ++ [R]); ss!.
+Qed.
+
+Lemma WellParen_epsilon
+  : WellParen [].
+Proof.
+  econs.
+  - ss!.
+  - intros ? H_prefix. inv H_prefix. destruct s_prefix as [ | [ | ] xs], s_suffix as [ | [ | ] ys]; s!; congruence || lia.
+Qed.
+
+Lemma WellParen_paren s
+  (WELLPAREN : WellParen s)
+  : WellParen ([L] ++ s ++ [R]).
+Proof with eauto.
+  econs.
+  - ss!.
+  - destruct WELLPAREN. intros xs Hxs. inv Hxs. destruct xs as [ | [ | ] s_prefix]; s!; try congruence || lia.
+    induction s_suffix as [ | [ | ] s_suffix _] using rev_ind; s!.
+    { apply L.app_cancel_l with (prefix := [L]) in H0. subst s_prefix. s!. lia. }
+    { enough (R = L) by congruence.
+      assert (H_view : R = last (L :: s ++ [R]) R).
+      { rewrite L.last_cons. rewrite L.last_last... }
+      assert (H_view' : L = last (L :: (s_prefix ++ s_suffix) ++ [L]) R).
+      { rewrite L.last_cons. rewrite L.last_last... }
+      congruence.
+    }
+    { apply L.app_cancel_l with (prefix := [L]) in H0.
+      apply L.app_cancel_r with (suffix := [R]) in H0.
+      exploit (PREFIX s_prefix); ss!.
+    }
+Qed.
+
+Lemma WellParen_concat s1 s2
+  (WELLPAREN1 : WellParen s1)
+  (WELLPAREN2 : WellParen s2)
+  : WellParen (s1 ++ s2).
+Proof.
+  destruct WELLPAREN1 as [H1H1 H1H2], WELLPAREN2 as [H2H1 H2H2]. econs.
+  - s!. lia.
+  - ii. pose proof (isPrefixOf_inv H_prefix) as [PREFIX | (s' & H_s_prefix & NOT_NIL & PREFIX')].
+    + ss!.
+    + subst s_prefix. s!.
+      enough (count L s' >= count R s') by lia.
+      ss!.
+Qed.
+
+#[local] Hint Resolve WellParen_epsilon WellParen_paren WellParen_concat : core.
+
+Theorem cfg2_equiv_WellParen (s : string)
+  : s \in L_cfg2 <-> WellParen s.
+Proof.
+  split.
+  { intros H_in. induction H_in; eauto. }
+  pose proof (relation_on_image_liftsWellFounded lt (@length alphabet) lt_wf s) as H_ACC.
+  induction H_ACC as [s _ IH]. change (forall s' : string, length s' < length s -> WellParen s' -> s' \in L_cfg2) in IH.
+  intros WELLPAREN. destruct s as [ | [ | ] s]; cycle -1.
+  { inv WELLPAREN. exploit (PREFIX [R]); ss!. change ([R] \prefix [R] ++ s). econs. }
+  { econs 1. }
+  set (w := L :: s) in *.
+  set (P := fun i : nat => i > 0 /\ count L (L.firstn i w) = count R (L.firstn i w)).
+  assert (P_dec : forall i, {P i} + {~ P i}).
+  { intros [ | n].
+    - right. unfold P. intros [? ?]; lia.
+    - set (i := S n) in *. pose proof (Nat.eq_dec (count L (L.firstn i w)) (count R (L.firstn i w))) as [YES | NO]; [left | right]; unfold P; lia.
+  }
+  exploit (dec_finds_minimum_if_exists P P_dec).
+  { exists (length w). red. rewrite firstn_all. split; [cbn; lia | inv WELLPAREN; eauto]. }
+  intros (j & H_j & MIN). change (forall i : nat, P i -> i >= j) in MIN.
+  rewrite <- firstn_skipn with (n := j) (l := w). econs 3.
+  - destruct H_j as [POS count_L_eq_count_R]. remember (L.firstn j w) as u eqn: H_u.
+    assert (claim1 : forall v, v \prefix u -> length v > 0 -> length v < length u -> count L v > count R v).
+    { intros v H_v H1_len_v H2_len_v.
+      assert (H_prefix : v \prefix w).
+      { transitivity u; [eauto | subst u; eapply firstn_isPrefixOf]. }
+      assert (count L v >= count R v) as Hge.
+      { destruct WELLPAREN. now eapply PREFIX. }
+      enough (count L v <> count R v) by lia.
+      intros H_contra.
+      enough (length v >= j) by now rewrite H_u in H2_len_v; rewrite length_firstn in H2_len_v; lia.
+      eapply MIN. split; eauto. replace (L.firstn (length v) w) with v; eauto.
+      symmetry. inv H_prefix. rewrite firstn_app. replace (length v - length v)%nat with 0%nat by lia.
+      simpl. rewrite app_nil_r. eapply firstn_all.
+    }
+    induction u as [ | [ | ] u _] using rev_ind.
+    { destruct j as [ | n]; [lia | now subst w; simpl in *]. }
+    { subst w. s!. destruct u as [ | [ | ] u].
+      - s!. lia.
+      - s!. exploit (claim1 (L :: u)).
+        { eapply app_isPrefixOf with (s := [L]). econs. }
+        { s!. lia. }
+        { s!. lia. }
+        intros HH. s!. exfalso; lia.
+      - destruct j as [ | n]; s!; [lia | congruence].
+    }
+    { subst w. destruct j as [ | n]; s!; [lia | ]. destruct u as [ | [ | ] u]; s!; try congruence.
+      econs 2. eapply IH.
+      - apply L.app_cancel_l with (prefix := [L]) in H_u.
+        pose proof (f_equal (@length alphabet) H_u). s!. lia.
+      - econs.
+        + lia.
+        + intros ? H_prefix.
+          assert (length s_prefix = 0 \/ length s_prefix > 0) as [NIL | NOT_NIL] by lia.
+          { destruct s_prefix; s!; [lia | exfalso; lia]. }
+          assert (length s_prefix < length u \/ length s_prefix >= length u) as [NOT_FULL | FULL] by lia.
+          { enough (count L (L :: s_prefix) > count R (L :: s_prefix)) by now s!; lia. eapply claim1.
+            - eapply app_isPrefixOf with (s := [L]). transitivity u; eauto. econs.
+            - s!. lia.
+            - s!. lia.
+          }
+          { inv H_prefix. destruct s_suffix; s!; lia. }
+    }
+  - destruct H_j as [POS count_L_eq_count_R]. eapply IH.
+    + rewrite length_skipn. subst w. s!. destruct j; lia.
+    + destruct WELLPAREN as [H1 H2]. econs.
+      { rewrite <- firstn_skipn with (n := j) (l := w) in H1. s!. lia. }
+      { intros s_prefix H_prefix. exploit (H2 (L.firstn j w ++ s_prefix)).
+        - rewrite <- firstn_skipn with (n := j) (l := w) at 2. now eapply app_isPrefixOf with (s := L.firstn j w).
+        - s!. lia.
+      }
+Qed.
+
+End THEORY.
 
 End LANG2.
